backend/Selectionproof.v
@@ -125,14 +125,6 @@ Lemma symbols_preserved:
   forall (s: ident), Genv.find_symbol tge s = Genv.find_symbol ge s.
 Proof. apply Senv.find_symbol_match_id. Qed.
 
-(*
-Lemma function_ptr_translated:
-  forall (b: block) (f: Cminor.fundef),
-  Genv.find_funct_ptr ge b = Some f ->
-  exists cu tf, Genv.find_funct_ptr tge b = Some tf /\ match_fundef cu f tf /\ linkorder cu prog.
-Proof. exact (Genv.find_funct_ptr_match TRANSF). Qed.
-*)
-
 Lemma functions_translated:
   forall (v v': val) (f: Cminor.fundef),
   Genv.find_funct ge v = Some f ->
